Sharing Prelim and definition of PCP

FOL/PCP.v
@@ -1,58 +1,6 @@
 (** * Post Correspondence Problem *)
 
-Require Export Reductions.
-
-(** ** Traditional Definition *)
-
-Definition symbol := nat.
-Definition string X := list X.
-Definition card X : Type := string X * string X.
-Definition stack X := list (card X).
-Definition SRS := stack nat.
-Definition BSRS := stack bool.
-
-Notation "x / y" := (x,y).
-
-Fixpoint tau1 (X : Type) (A : stack X) : string X :=
-  match A with
-  | [] => []
-  | (x / y) :: A => x ++ tau1 A
-  end.
-
-Fixpoint tau2 X (A : stack X) : string X :=
-  match A with
-  | [] => []
-  | (x / y) :: A => y ++ tau2 A
-  end.
-
-Definition PCP P := exists A : SRS, A <<= P /\ A <> [] /\ tau1 A = tau2 A.
-
-(** ** Inductive Definition *)
-
-Inductive derivable (X : Type) (R : stack X) : string X -> string X -> Prop :=
-|  der_sing x y : x/y el R -> derivable R x y
-| der_cons x y u v : x/y el R -> derivable R u v -> derivable R (x ++ u) (y ++ v).
-
-Lemma derivable_BPCP X (P : stack X) u v :
-  derivable P u v -> exists A, A <<= P /\ A <> nil /\ tau1 A = u /\ tau2 A = v.
-Proof.
-  induction 1 as [ | ? ? ? ? ? ? (A & ? & ? & ? & ?)].
-  - exists [x/y]. repeat split; cbn; simpl_list; eauto. congruence.
-  - subst. exists (x/y :: A). repeat split. eauto. congruence.
-Qed.
-    
-Lemma BPCP_derivable X (P : stack X) u v : (exists A, A <<= P /\ A <> nil /\ tau1 A = u /\ tau2 A = v) -> derivable P u v.
-Proof.
-  intros (A & ? & ? & ? & ?). subst. 
-  revert H. pattern A. revert A H0. eapply list_ind_ne; cbn; intros; destruct x as (x,y).
-  - simpl_list. eauto using derivable.
-  - eauto using derivable.
-Qed.
-
-(** ** Binary PCP *)
-
-Inductive BPCP P : Prop := cBPCP u (_ : @derivable bool P u u).
-Hint Constructors BPCP.
+Require Export Reductions Problems.PCP.
 
 Lemma stack_discrete :
   discrete (stack bool).
@@ -100,7 +48,7 @@ Proof.
   eapply enum_count. intros; repeat decide equality. eapply enum_PCP'.
 Qed.
 
-Lemma enumerable_PCP : enumerable BPCP.
+Lemma enumerable_PCP : enumerable BPCP'.
 Proof.
   pose proof enumerable_derivable. 
   assert (enumerable (X := (stack bool * (string bool * string bool))) (fun '(C, (s, t)) => s = t)). {
