Makefile
@@ -6,7 +6,7 @@ html: Makefile.coq
 
 clean: Makefile.coq
 	+make -f Makefile.coq clean
-	rm -f Makefile.coq
+	rm -f Makefile.coq Makefile.coq.conf
 
 Makefile.coq: _CoqProject
 	coq_makefile -f _CoqProject -o Makefile.coq
